list comprehension works

src/Inflist.v
@@ -7,6 +7,7 @@ Require Import AST.
 Require Import Semantics.
 Require Import Utils.
 Require Import Builtins.
+Require Import Tactics.
 
 Import HaskellListNotations.
 Open Scope string_scope.
@@ -19,6 +20,8 @@ Definition inflist := (NonRecursive
                                             (ETApp (ETApp (EVar 0) (TCon (TC (TCNum 2)) [])) (TCon (TC (TCNum 8)) [])))))).
 
 Definition finlist := (NonRecursive (Decl 246 (DExpr (EList [(ETApp (ETApp (EVar 0) (TCon (TC (TCNum 1)) [])) (TCon (TC (TCNum 8)) [])),(ETApp (ETApp (EVar 0) (TCon (TC (TCNum 2)) [])) (TCon (TC (TCNum 8)) [])),(ETApp (ETApp (EVar 0) (TCon (TC (TCNum 3)) [])) (TCon (TC (TCNum 8)) []))])))).
+
+Definition finlist_sel_exp := ESel (EVar 246) (ListSel ((ETApp (ETApp (EVar 0) (TCon (TC (TCNum 2)) [])) (TCon (TC (TCNum 8)) [])))).
 
 Definition elem := (NonRecursive (Decl 247 (DExpr (EApp (EApp (ETApp (ETApp (ETApp (EVar 40) (TCon (TC (TCNum 3)) [])) (TCon (TC TCSeq) [TCon (TC (TCNum 8)) [],TCon (TC TCBit) []])) (TCon (TC (TCNum 1)) [])) (EVar 246)) (ETApp (ETApp (EVar 0) (TCon (TC (TCNum 1)) [])) (TCon (TC (TCNum 1)) [])))))).
 
@@ -68,3 +71,96 @@ Proof.
   Unshelve.
   all: unfold Z.to_nat; unfold Pos.to_nat; simpl; try congruence.
 Qed.
+
+Definition one := bits (@repr 8 nz 1).
+Definition two := bits (@repr 8 nz 2).
+
+Lemma finlist_sel_eval :
+  eval_expr (bind_decl_group finlist gempty) empty finlist_sel_exp three.
+Proof.
+  e. e.
+  match goal with
+  | [ |- select_list _ _ ?N _ _ ] => replace N with (S (S O)) by (simpl; reflexivity)
+  end.
+  econstructor.
+  global. e.
+  repeat econstructor. simpl. reflexivity.
+  econstructor. econstructor. unfold extend. simpl. reflexivity.
+  econstructor. econstructor. simpl. reflexivity.
+  Unshelve.
+  all: exact nz.
+Qed.
+
+
+Definition where_decl := (NonRecursive (Decl 250 (DExpr (EWhere (EVar 259) [(NonRecursive (Decl 259 (DExpr (ETApp (ETApp (EVar 0) (TCon (TC (TCNum 3)) [])) (TCon (TC (TCNum 8)) [])))))])))).
+
+Lemma where_eval :
+  eval_expr (bind_decl_group where_decl gempty) empty (EVar 250) three.
+Proof.
+  global.
+  e. e. global.
+  e.
+Qed.
+
+Definition listcomp := (NonRecursive (Decl 251 (DExpr (EAbs 261 (EWhere (EVar 262) [(NonRecursive (Decl 262 (DExpr (EComp (EApp (EApp (ETApp (EVar 1) (TCon (TC TCSeq) [TCon (TC (TCNum 8)) [],TCon (TC TCBit) []])) (EVar 263)) (EVar 264)) [[(From 263 (EVar 261))],[(From 264 (EList [(ETApp (ETApp (EVar 0) (TCon (TC (TCNum 1)) [])) (TCon (TC (TCNum 8)) [])),(ETApp (ETApp (EVar 0) (TCon (TC (TCNum 2)) [])) (TCon (TC (TCNum 8)) [])),(ETApp (ETApp (EVar 0) (TCon (TC (TCNum 3)) [])) (TCon (TC (TCNum 8)) [])),(ETApp (ETApp (EVar 0) (TCon (TC (TCNum 4)) [])) (TCon (TC (TCNum 8)) []))]))]]))))]))))). 
+
+Definition comp_idx_expr : Expr := ESel (EApp (EVar 251) (EVar 246)) (ListSel (ETApp (ETApp (EVar 0) (TCon (TC (TCNum 2)) [])) (TCon (TC (TCNum 8)) []))).
+
+Definition six := bits (@repr 8 nz 6).
+
+Lemma listcomp_eval :
+  eval_expr (bind_decl_groups (listcomp :: finlist :: plus_decl :: nil) gempty) empty comp_idx_expr six.
+Proof.
+  unfold comp_idx_expr.
+  e.
+  e.
+  eapply select_comp.
+  e. global. e. global. e.
+  repeat econstructor. e.
+  global. e.
+  
+  econstructor. econstructor.
+  econstructor.
+  econstructor. simpl. reflexivity.
+
+  econstructor. econstructor.
+  reflexivity.
+  eapply select_zero. econstructor. reflexivity.
+  econstructor. econstructor. 
+  econstructor. econstructor.
+  
+  repeat econstructor. reflexivity.
+  econstructor. econstructor. reflexivity.
+  econstructor. econstructor. reflexivity.
+  econstructor. econstructor.
+  econstructor. e. global. econstructor. econstructor.
+  reflexivity.
+  econstructor. econstructor. reflexivity.
+  econstructor. econstructor. reflexivity.
+  econstructor. reflexivity.
+  econstructor. omega.
+  Unshelve.
+  all: exact nz.
+Qed.
+
+  
+Definition gf28Add := (NonRecursive (Decl 249 (DExpr (ETAbs 331 (EAbs 255 (EWhere (EApp (EApp (ETApp (ETApp (ETApp (EVar 42) (TCon (TF TCAdd) [TCon (TC (TCNum 1)) [],TVar (TVBound 331 KNum)])) (TCon (TC TCSeq) [TCon (TC (TCNum 8)) [],TCon (TC TCBit) []])) (TCon (TC (TCNum 0)) [])) (EVar 256)) (ETApp (ETApp (EVar 0) (TCon (TC (TCNum 0)) [])) (TCon (TC (TCNum 0)) []))) [(Recursive [(Decl 256 (DExpr (EApp (EApp (ETApp (ETApp (ETApp (EVar 34) (TCon (TC (TCNum 1)) [])) (TVar (TVBound 331 KNum))) (TCon (TC TCSeq) [TCon (TC (TCNum 8)) [],TCon (TC TCBit) []])) (EList [(ETApp (EVar 29) (TCon (TC TCSeq) [TCon (TC (TCNum 8)) [],TCon (TC TCBit) []]))])) (EComp (EApp (EApp (ETApp (EVar 28) (TCon (TC TCSeq) [TCon (TC (TCNum 8)) [],TCon (TC TCBit) []])) (EVar 257)) (EVar 258)) [[(From 257 (EVar 255))],[(From 258 (EVar 256))]]))))])])))))).
+
+Definition add_call := (NonRecursive (Decl 250 (DExpr (EApp (ETApp (EVar 249) (TCon (TC (TCNum 2)) [])) (EList [(ETApp (ETApp (EVar 0) (TCon (TC (TCNum 1)) [])) (TCon (TC (TCNum 8)) [])),(ETApp (ETApp (EVar 0) (TCon (TC (TCNum 2)) [])) (TCon (TC (TCNum 8)) []))]))))).
+
+Definition gf28_add_ge := bind_decl_groups (gf28Add :: add_call :: plus_decl :: nil) gempty.
+
+
+Lemma eval_gf28_add :
+  eval_expr gf28_add_ge empty (EVar 250) three.
+Proof.
+  unfold gf28_add_ge. unfold bind_decl_groups.
+  global.
+  e.
+  e. global.
+  e. e. e. repeat econstructor.
+  e. e. e. e. e. e. eapply eval_global_var.
+  unfold extend. simpl. reflexivity.
+  (* TODO *)
+  
+Admitted.  
